Refactor traces and small step semantics to take an event argument
Co-authored-by: Rob Blanco <roberto.blanco@inria.fr>

CompCert/Events.v
@@ -32,51 +32,51 @@ Definition next_comp_of_event (e: event) : Component.id :=
   | EWrite C _ _   => C
   end.
 
-Definition trace := list event.
+Definition trace (A : Type) := list A.
 
-Definition E0 : trace := nil.
+Definition E0 {A : Type} : trace A := nil.
 
-Definition Eapp (t1 t2: trace) : trace := t1 ++ t2.
+Definition Eapp {A : Type} (t1 t2: trace A) : trace A := t1 ++ t2.
 
-CoInductive traceinf : Type :=
-  | Econsinf: event -> traceinf -> traceinf.
+CoInductive traceinf (A : Type) : Type :=
+| Econsinf: A -> traceinf A -> traceinf A.
 
-Fixpoint Eappinf (t: trace) (T: traceinf) {struct t} : traceinf :=
+Fixpoint Eappinf {A : Type} (t: trace A) (T: traceinf A) {struct t} : traceinf A :=
   match t with
   | nil => T
-  | ev :: t' => Econsinf ev (Eappinf t' T)
+  | ev :: t' => Econsinf _ ev (Eappinf t' T)
   end.
 
 (** Concatenation of traces is written [**] in the finite case
-  or [***] in the infinite case. *)
+      or [***] in the infinite case. *)
 
 Infix "**" := Eapp (at level 60, right associativity).
 Infix "***" := Eappinf (at level 60, right associativity).
 
-Lemma E0_left: forall t, E0 ** t = t.
+Lemma E0_left: forall A (t: trace A), E0 ** t = t.
 Proof. auto. Qed.
 
-Lemma E0_right: forall t, t ** E0 = t.
+Lemma E0_right: forall A (t: trace A) , t ** E0 = t.
 Proof. intros. unfold E0, Eapp. rewrite <- app_nil_end. auto. Qed.
 
-Lemma Eapp_assoc: forall t1 t2 t3, (t1 ** t2) ** t3 = t1 ** (t2 ** t3).
+Lemma Eapp_assoc: forall A (t1: trace A) t2 t3, (t1 ** t2) ** t3 = t1 ** (t2 ** t3).
 Proof. intros. unfold Eapp, trace. apply app_ass. Qed.
 
-Lemma Eapp_E0_inv: forall t1 t2, t1 ** t2 = E0 -> t1 = E0 /\ t2 = E0.
+Lemma Eapp_E0_inv: forall A (t1: trace A) t2, t1 ** t2 = E0 -> t1 = E0 /\ t2 = E0.
 Proof.
   intros. apply app_eq_nil. auto.
 Qed.
 
-Lemma E0_left_inf: forall T, E0 *** T = T.
+Lemma E0_left_inf: forall A (T : @traceinf A) , E0 *** T = T.
 Proof. auto. Qed.
 
-Lemma Eappinf_assoc: forall t1 t2 T, (t1 ** t2) *** T = t1 *** (t2 *** T).
+Lemma Eappinf_assoc: forall A (t1: trace A) t2 T, (t1 ** t2) *** T = t1 *** (t2 *** T).
 Proof.
   induction t1; intros; simpl. auto. decEq; auto.
 Qed.
 
 Hint Rewrite E0_left E0_right Eapp_assoc
-             E0_left_inf Eappinf_assoc: trace_rewrite.
+     E0_left_inf Eappinf_assoc: trace_rewrite.
 
 Opaque trace E0 Eapp Eappinf.
 
@@ -85,16 +85,16 @@ Opaque trace E0 Eapp Eappinf.
 
 Ltac substTraceHyp :=
   match goal with
-  | [ H: (@eq trace ?x ?y) |- _ ] =>
-       subst x || clear H
+  | [ H: (@eq (trace _) ?x ?y) |- _ ] =>
+    subst x || clear H
   end.
 
 Ltac decomposeTraceEq :=
   match goal with
   | [ |- (_ ** _) = (_ ** _) ] =>
-      apply (f_equal2 Eapp); auto; decomposeTraceEq
+    apply (f_equal2 Eapp); auto; decomposeTraceEq
   | _ =>
-      auto
+    auto
   end.
 
 Ltac traceEq :=
@@ -102,42 +102,42 @@ Ltac traceEq :=
 
 (** Bisimilarity between infinite traces. *)
 
-CoInductive traceinf_sim: traceinf -> traceinf -> Prop :=
-  | traceinf_sim_cons: forall e T1 T2,
-      traceinf_sim T1 T2 ->
-      traceinf_sim (Econsinf e T1) (Econsinf e T2).
+CoInductive traceinf_sim {A : Type} : traceinf A -> traceinf A -> Prop :=
+| traceinf_sim_cons: forall e T1 T2,
+    traceinf_sim T1 T2 ->
+    traceinf_sim (Econsinf _ e T1) (Econsinf _ e T2).
 
 Lemma traceinf_sim_refl:
-  forall T, traceinf_sim T T.
+  forall A (T : traceinf A), traceinf_sim T T.
 Proof.
   cofix COINDHYP; intros.
   destruct T. constructor. apply COINDHYP.
 Qed.
 
 Lemma traceinf_sim_sym:
-  forall T1 T2, traceinf_sim T1 T2 -> traceinf_sim T2 T1.
+  forall A (T1 : traceinf A) T2, traceinf_sim T1 T2 -> traceinf_sim T2 T1.
 Proof.
   cofix COINDHYP; intros. inv H; constructor; auto.
 Qed.
 
 Lemma traceinf_sim_trans:
-  forall T1 T2 T3,
-  traceinf_sim T1 T2 -> traceinf_sim T2 T3 -> traceinf_sim T1 T3.
+  forall A (T1 : traceinf A) T2 T3,
+    traceinf_sim T1 T2 -> traceinf_sim T2 T3 -> traceinf_sim T1 T3.
 Proof.
   cofix COINDHYP;intros. inv H; inv H0; constructor; eauto.
 Qed.
 
-CoInductive traceinf_sim': traceinf -> traceinf -> Prop :=
-  | traceinf_sim'_cons: forall t T1 T2,
-      t <> E0 -> traceinf_sim' T1 T2 -> traceinf_sim' (t *** T1) (t *** T2).
+CoInductive traceinf_sim' {A : Type} : traceinf A -> traceinf A -> Prop :=
+| traceinf_sim'_cons: forall t T1 T2,
+    t <> E0 -> traceinf_sim' T1 T2 -> traceinf_sim' (t *** T1) (t *** T2).
 
 Lemma traceinf_sim'_sim:
-  forall T1 T2, traceinf_sim' T1 T2 -> traceinf_sim T1 T2.
+  forall A (T1 : traceinf A) T2, traceinf_sim' T1 T2 -> traceinf_sim T1 T2.
 Proof.
   cofix COINDHYP; intros. inv H.
   destruct t. elim H0; auto.
-Transparent Eappinf.
-Transparent E0.
+  Transparent Eappinf.
+  Transparent E0.
   simpl.
   destruct t. simpl. constructor. apply COINDHYP; auto.
   constructor. apply COINDHYP.
@@ -147,14 +147,15 @@ Qed.
 (** An alternate presentation of infinite traces as
   infinite concatenations of nonempty finite traces. *)
 
-CoInductive traceinf': Type :=
-  | Econsinf': forall (t: trace) (T: traceinf'), t <> E0 -> traceinf'.
+CoInductive traceinf' (A : Type) : Type :=
+| Econsinf': forall (t: trace A) (T: traceinf' A), t <> E0 -> traceinf' A.
 
-Program Definition split_traceinf' (t: trace) (T: traceinf') (NE: t <> E0): event * traceinf' :=
+Program Definition split_traceinf' {A : Type} (t: trace A) (T: traceinf' A) (NE: t <> E0)
+  : A * traceinf' A :=
   match t with
   | nil => _
   | e :: nil => (e, T)
-  | e :: t' => (e, Econsinf' t' T _)
+  | e :: t' => (e, Econsinf' _ t' T _)
   end.
 Next Obligation.
   elimtype False. elim NE. auto.
@@ -163,58 +164,58 @@ Next Obligation.
   red; intro. elim (H e). rewrite H0. auto.
 Qed.
 
-CoFixpoint traceinf_of_traceinf' (T': traceinf') : traceinf :=
+CoFixpoint traceinf_of_traceinf' {A : Type} (T': traceinf' A) : traceinf A :=
   match T' with
   | Econsinf' t T'' NOTEMPTY =>
-      let (e, tl) := split_traceinf' t T'' NOTEMPTY in
-      Econsinf e (traceinf_of_traceinf' tl)
+    let (e, tl) := split_traceinf' t T'' NOTEMPTY in
+    Econsinf _ e (traceinf_of_traceinf' tl)
   end.
 
 Remark unroll_traceinf':
-  forall T, T = match T with Econsinf' t T' NE => Econsinf' t T' NE end.
+  forall A (T : traceinf' A), T = match T with Econsinf' t T' NE => Econsinf' _ t T' NE end.
 Proof.
   intros. destruct T; auto.
 Qed.
 
 Remark unroll_traceinf:
-  forall T, T = match T with Econsinf t T' => Econsinf t T' end.
+  forall {A} (T: traceinf A), T = match T with Econsinf t T' => Econsinf _ t T' end.
 Proof.
   intros. destruct T; auto.
 Qed.
 
 Lemma traceinf_traceinf'_app:
-  forall t T NE,
-  traceinf_of_traceinf' (Econsinf' t T NE) = t *** traceinf_of_traceinf' T.
+  forall {A} (t: trace A) T NE,
+    traceinf_of_traceinf' (Econsinf' _ t T NE) = t *** traceinf_of_traceinf' T.
 Proof.
   induction t.
   intros. elim NE. auto.
   intros. simpl.
-  rewrite (unroll_traceinf (traceinf_of_traceinf' (Econsinf' (a :: t) T NE))).
+  rewrite (unroll_traceinf (traceinf_of_traceinf' (Econsinf' _ (a :: t) T NE))).
   simpl. destruct t. auto.
-Transparent Eappinf.
+  Transparent Eappinf.
   simpl. f_equal. apply IHt.
 Qed.
 
 (** Prefixes of traces. *)
 
-Definition trace_prefix (t1 t2: trace) :=
+Definition trace_prefix {A : Type} (t1 t2: trace A) :=
   exists t3, t2 = t1 ** t3.
 
-Definition traceinf_prefix (t1: trace) (T2: traceinf) :=
+Definition traceinf_prefix {A : Type} (t1: trace A) (T2: traceinf A) :=
   exists T3, T2 = t1 *** T3.
 
 Lemma trace_prefix_app:
-  forall t1 t2 t,
-  trace_prefix t1 t2 ->
-  trace_prefix (t ** t1) (t ** t2).
+  forall {A} (t1 : trace A) t2 t,
+    trace_prefix t1 t2 ->
+    trace_prefix (t ** t1) (t ** t2).
 Proof.
   intros. destruct H as [t3 EQ]. exists t3. traceEq.
 Qed.
 
 Lemma traceinf_prefix_app:
-  forall t1 T2 t,
-  traceinf_prefix t1 T2 ->
-  traceinf_prefix (t ** t1) (t *** T2).
+  forall {A} (t1: trace A) T2 t,
+    traceinf_prefix t1 T2 ->
+    traceinf_prefix (t ** t1) (t *** T2).
 Proof.
   intros. destruct H as [T3 EQ]. exists T3. subst T2. traceEq.
 Qed.
@@ -224,7 +225,7 @@ Set Implicit Arguments.
 (* TODO: What does match_traces mean? How should it be updated now
    that we have ERead and EWrite?
  *)
-Inductive match_traces: trace -> trace -> Prop :=
+Inductive match_traces: (@trace event) -> (@trace event) -> Prop :=
   | match_traces_E0:
       match_traces nil nil
   | match_traces_call: forall C P arg C',
